LeanSubst/Types/Option.lean
@@ -9,17 +9,17 @@ variable {V : List (Type u2)}
 
 def Option.rmap [RenMap S V] (r : RenVec V) : Option S -> Option S
 | none => none
-| some t => some t⟨;r⟩
+| some t => some t⟨r,⟩
 
 instance [RenMap S V] : RenMap (Option S) V where
   rmap := Option.rmap
 
 @[simp, grind =]
-theorem Option.rmap_none [RenMap S V] {r : RenVec V} : (@Option.none S)⟨;r⟩ = none := by
+theorem Option.rmap_none [RenMap S V] {r : RenVec V} : (@Option.none S)⟨r,⟩ = none := by
   simp [RenMap.rmap, Option.rmap]
 
 @[simp, grind =]
-theorem Option.rmap_some [RenMap S V] {x : S} {r : RenVec V} : (some x)⟨;r⟩ = some x⟨;r⟩ := by
+theorem Option.rmap_some [RenMap S V] {x : S} {r : RenVec V} : (some x)⟨r,⟩ = some x⟨r,⟩ := by
   simp [RenMap.rmap, Option.rmap]
 
 instance [RenMap S V] [RenMapId S V] : RenMapId (Option S) V where
@@ -30,17 +30,17 @@ instance [RenMap S V] [RenMapCompose S V] : RenMapCompose (Option S) V where
 
 def Option.smap [SubstMap S V] (σ : SubstVec V) : Option S -> Option S
 | none => none
-| some t => some t[;σ]
+| some t => some t[σ,]
 
 instance [SubstMap S V] : SubstMap (Option S) V where
   smap := Option.smap
 
 @[simp, grind =]
-theorem Option.smap_none [SubstMap S V] {σ : SubstVec V} : (@Option.none S)[;σ] = none := by
+theorem Option.smap_none [SubstMap S V] {σ : SubstVec V} : (@Option.none S)[σ,] = none := by
   simp [SubstMap.smap, Option.smap]
 
 @[simp, grind =]
-theorem Option.smap_some [SubstMap S V] {x : S} {σ : SubstVec V} : (some x)[;σ] = some x[;σ] := by
+theorem Option.smap_some [SubstMap S V] {x : S} {σ : SubstVec V} : (some x)[σ,] = some x[σ,] := by
   simp [SubstMap.smap, Option.smap]
 
 instance [RenMap S V] [SubstMap S V] [SubstMapId S V] : SubstMapId (Option S) V where
